txn-data-consistency/Key_Value_Stores.thy
@@ -4,6 +4,15 @@ theory Key_Value_Stores
   imports Event_Systems "HOL-Library.Sublist" Closedness
 begin
 
+
+subsection \<open>General lemmas about lists etc.\<close>
+
+lemma nth_append_length':
+  assumes "length xs = i" 
+  shows "(xs @ x # ys) ! i = x"
+  using assms[symmetric] by simp
+
+
 subsection \<open>Transaction IDs and session order\<close>
 
 typedecl cl_id
@@ -54,15 +63,64 @@ lemmas kvs_init_defs = kvs_init_def v_list_init_def version_init_def
 
 subsubsection \<open>Full view on a version list\<close>
 
-\<comment> \<open>index range for a kvs and key\<close>
+text \<open>The full view is the index range for a version list (or kvs and key)\<close>  
 
-definition full_view :: "('v, 'm) vs_list \<Rightarrow> nat set" where  
-  "full_view vl \<equiv> {..<length vl}"
+definition full_view :: "('v, 'm) vs_list \<Rightarrow> nat set" where   (* CHSP: DROP OR CHANGE THIS DEF? *)
+  "full_view vl = {..<length vl}"
+
+lemma full_view_elemI [intro]: "i < length vl \<Longrightarrow> i \<in> full_view vl"    (* AUT-ADDED *)
+  by (simp add: full_view_def)
+
+lemma full_view_elemD: "i \<in> full_view vl \<Longrightarrow> i < length vl"
+  by (simp add: full_view_def)
 
 thm nth_list_update_eq nth_list_update_neq
 
+
+text \<open>Full view as set\<close>
+
 lemma full_view_finite [simp, intro!]: "finite (full_view vl)"
   by (simp add: full_view_def)
+
+lemma full_view_eq_is_length_eq [simp]: 
+  "full_view vl = full_view vl' \<longleftrightarrow> length vl = length vl'"
+  by (simp add: full_view_def)
+
+lemma full_view_subset_is_length_leq: 
+  "full_view vl \<subseteq> full_view vl' \<longleftrightarrow> length vl \<le> length vl'"
+  by (simp add: full_view_def)
+
+lemma full_view_snoc [simp]:  
+  "full_view (vl @ [ver]) = insert (length vl) (full_view vl)"
+  by (auto simp add: full_view_def)
+
+lemma full_view_vl_update [simp]:
+  "full_view (vl[i := ver]) = full_view vl"
+  by (simp)
+
+lemma full_view_update_append [simp]:
+  "full_view (vl[i := x] @ vs) = full_view (vl @ vs)"
+  by (simp)
+
+
+text \<open>Elements of full view\<close>
+
+lemma zero_in_full_view [simp]: "vl \<noteq> [] \<Longrightarrow> 0 \<in> full_view vl"         (* AUT-ADDED *)
+  by (simp add: full_view_def)
+
+lemma max_in_full_view [simp]: "vl \<noteq> [] \<Longrightarrow> Max (full_view vl) \<in> full_view vl"
+  using Max_in zero_in_full_view by auto
+
+lemma full_view_grows: 
+  "i \<in> full_view vl \<Longrightarrow> i \<in> full_view (vl @ vs)"
+  by (simp add: full_view_def)
+
+lemma full_view_kvs_init [simp]:
+  "i \<in> full_view (kvs_init k) \<longleftrightarrow> i = 0"
+  by (simp add: kvs_init_defs full_view_def)
+
+
+text \<open>Indexing version list elements in full view\<close>
 
 lemma full_view_nth_list_update_eq [simp]:     (* special case of nth_list_update_eq *)
   "i \<in> full_view vl \<Longrightarrow> vl[i := x] ! i = x"
@@ -72,47 +130,43 @@ lemma full_view_append [simp]:
   "i \<in> full_view vl \<Longrightarrow> (vl @ vs) ! i = vl ! i"
   by (auto simp add: full_view_def nth_append)
 
-lemma full_view_update [simp]:
-  "full_view (vl [i := x]) = full_view vl"
-  by (simp add: full_view_def)
 
-lemma full_view_update_append [simp]:
-  "full_view (vl[i := x] @ vs) = full_view (vl @ vs)"
-  by (simp add: full_view_def)
 
-lemma full_view_grows: 
-  "i \<in> full_view vl \<Longrightarrow> i \<in> full_view (vl @ vs)"
-  by (simp add: full_view_def)
+lemma full_view_length_increasing:    (* REMOVE? *)
+  assumes "length vl \<le> length vl'"
+    and "i \<in> full_view vl"
+  shows "i \<in> full_view vl'"
+  using assms by (simp add: full_view_def)
 
-lemma zero_in_full_view:
-  " vl\<noteq> [] \<Longrightarrow> 0 \<in> full_view vl"
-  by (simp add: full_view_def)
 
-lemma full_view_kvs_init [simp]:
-  "i \<in> full_view (kvs_init k) \<longleftrightarrow> i = 0"
-  by (simp add: kvs_init_defs full_view_def)
-  
+lemma full_view_same_length:          (* REMOVE? *)
+  assumes "length vl = length vl'"
+    and "i \<in> full_view vl"
+  shows "i \<in> full_view vl'"
+  using assms by (simp add: full_view_def)
+
+
+
+
+
+
+
+
+
+
+(* SUBSUMED BY LEMMA full_view_snoc:
+
 lemma length_vl_in_appended:
   "length vl \<in> full_view (vl @ [v])"
-  by (simp add: full_view_def)
+  by (simp)
 
 lemma full_view_x_in_append [simp]:
   assumes "i \<in> full_view (vl @ [v])"
     and "i \<notin> full_view vl"
   shows "i = length vl"
   using assms by (simp add: full_view_def)
+*)
 
-lemma full_view_same_length:
-  assumes "length vl = length vl'"
-    and "i \<in> full_view vl"
-  shows "i \<in> full_view vl'"
-  using assms by (simp add: full_view_def)
-
-lemma full_view_length_increasing:
-  assumes "length vl \<le> length vl'"
-    and "i \<in> full_view vl"
-  shows "i \<in> full_view vl'"
-  using assms by (simp add: full_view_def)
 
 (*
   TODO: there are too many uses of full_view_def below; 
@@ -129,15 +183,28 @@ definition snapshot_property :: "('v, 'm) kvs_store \<Rightarrow> bool" where
 lemmas snapshot_propertyI = snapshot_property_def [THEN iffD2, rule_format]
 lemmas snapshot_propertyE [elim] = snapshot_property_def [THEN iffD1, elim_format, rule_format]
 
+lemma snapshot_propertyD1:
+    "\<lbrakk> t \<in> v_readerset (K k ! i); t \<in> v_readerset (K k ! j);
+       i \<in> full_view (K k); j \<in> full_view (K k); snapshot_property K \<rbrakk> 
+   \<Longrightarrow> i = j"
+  by (auto simp add: snapshot_property_def)
+
+lemma snapshot_propertyD2:
+    "\<lbrakk> v_writer (K k ! i) = v_writer (K k ! j); 
+       i \<in> full_view (K k); j \<in> full_view (K k); snapshot_property K \<rbrakk> 
+   \<Longrightarrow> i = j"
+  by (auto simp add: snapshot_property_def)
+
 lemma snapshot_property_kvs_init [simp, intro]: "snapshot_property kvs_init"
   by (intro snapshot_propertyI) (auto)
 
 definition wr_so :: "('v, 'm) kvs_store \<Rightarrow> bool" where
   "wr_so K \<longleftrightarrow> (\<forall>k t t'. \<forall>i \<in> full_view (K k).
-                  t = v_writer (K k!i) \<and> t' \<in> Tn ` v_readerset (K k!i) \<longrightarrow> (t', t) \<notin> SO^=)"
+                  t = v_writer (K k!i) \<longrightarrow> t' \<in> Tn ` v_readerset (K k!i) \<longrightarrow> (t', t) \<notin> SO^=)"
 
 lemmas wr_soI = wr_so_def [THEN iffD2, rule_format]
 lemmas wr_soE [elim] = wr_so_def [THEN iffD1, elim_format, rule_format]
+lemmas wr_soD = wr_so_def [THEN iffD1, rule_format]
 
 lemma wr_so_kvs_init [simp, intro]: "wr_so kvs_init"
   by (intro wr_soI) (auto simp add: kvs_init_defs full_view_def)
@@ -145,10 +212,11 @@ lemma wr_so_kvs_init [simp, intro]: "wr_so kvs_init"
 
 definition ww_so :: "('v, 'm) kvs_store \<Rightarrow> bool" where
   "ww_so K \<longleftrightarrow> (\<forall>k t t'. \<forall>i \<in> full_view (K k). \<forall>j \<in> full_view (K k).
-                  t = v_writer (K k!i) \<and> t' = v_writer (K k!j) \<and> i < j \<longrightarrow> (t', t) \<notin> SO^=)"
+                  t = v_writer (K k!i) \<longrightarrow> t' = v_writer (K k!j) \<longrightarrow> i < j \<longrightarrow> (t', t) \<notin> SO^=)"
 
 lemmas ww_soI = ww_so_def [THEN iffD2, rule_format]
 lemmas ww_soE [elim] = ww_so_def [THEN iffD1, elim_format, rule_format]
+lemmas ww_soD = ww_so_def [THEN iffD1, rule_format]
 
 lemma ww_so_kvs_init [simp, intro]: "ww_so kvs_init"
   by (intro ww_soI) (auto simp add: kvs_init_defs full_view_def)
@@ -240,8 +308,8 @@ lemma fresh_txid_v_writer:
     and "i \<in> full_view (K k)"
   shows "v_writer (K k!i) \<noteq> Tn t"
   using assms nth_mem
-  apply (auto simp add: fresh_txid_defs image_iff full_view_def)
-  by fastforce
+  apply (auto 4 3 simp add: fresh_txid_defs image_iff full_view_def)
+  by (fastforce)
 
 lemma fresh_txid_v_reader_set:
   assumes "t \<in> next_txids K cl"
@@ -260,6 +328,7 @@ lemma fresh_txid_writer_so:
   by fastforce
 
 
+
 subsection \<open>Views\<close>
 
 type_synonym v_id = nat
@@ -270,8 +339,29 @@ type_synonym view = "key \<Rightarrow> key_view"
 definition view_init :: view where
   "view_init \<equiv> (\<lambda>k. {0})"
 
+
+subsubsection \<open>View order\<close>
+
 definition view_order (infix "\<sqsubseteq>" 60) where
   "u1 \<sqsubseteq> u2 \<equiv> \<forall>k. u1 k \<subseteq> u2 k"
+
+lemma view_order_refl: "u \<sqsubseteq> u"
+  by (simp add: view_order_def)
+
+lemma view_order_trans: "\<lbrakk> u1 \<sqsubseteq> u2; u2 \<sqsubseteq> u3 \<rbrakk> \<Longrightarrow> u1 \<sqsubseteq> u3"
+  by (auto simp add: view_order_def)
+
+lemma view_order_full_view_increasing:
+  assumes "\<And>k. length (K k) \<le> length (K' k)"
+  shows "(full_view o K) \<sqsubseteq> (full_view o K')"
+  using assms
+  by (simp add: full_view_def view_order_def)
+
+
+
+subsubsection \<open>View well-formedness\<close>
+
+text \<open>View in range\<close>
 
 definition key_view_in_range :: "('v, 'm) vs_list \<Rightarrow> key_view \<Rightarrow> bool" where
   "key_view_in_range vl uk \<equiv> 0 \<in> uk \<and> uk \<subseteq> full_view vl"
@@ -280,21 +370,6 @@ definition view_in_range :: "('v, 'm) kvs_store \<Rightarrow> view \<Rightarrow>
   "view_in_range K u \<equiv> \<forall>k. key_view_in_range (K k) (u k)"
 
 lemmas view_in_range_defs = view_in_range_def key_view_in_range_def
-
-definition view_atomic :: "('v, 'm) kvs_store \<Rightarrow> view \<Rightarrow> bool" where
-  "view_atomic K u \<equiv> \<forall>k k'.  \<forall>i \<in> u k. \<forall>i' \<in> full_view (K k').
-    v_writer (K k!i) = v_writer (K k'!i') \<longrightarrow> i' \<in> u k'"
-
-definition view_wellformed :: "('v, 'm) kvs_store \<Rightarrow> view \<Rightarrow> bool" where
-  "view_wellformed K u \<longleftrightarrow> view_in_range K u \<and> view_atomic K u"
-
-lemmas view_wellformedD1 [dest] = view_wellformed_def [THEN iffD1, THEN conjunct1]
-lemmas view_wellformedD2 [dest] = view_wellformed_def [THEN iffD1, THEN conjunct2]
-
-lemmas view_wellformed_defs = 
-  view_wellformed_def view_in_range_defs view_atomic_def 
-
-\<comment> \<open>key_view lemmas\<close>
 
 lemma key_view_non_empty [simp]:
   assumes "key_view_in_range vl uk"
@@ -321,30 +396,6 @@ lemma key_view_zero_full_view:
   shows "0 \<in> full_view vl" 
   using assms
   by (auto simp add: key_view_in_range_def)
-
-lemma full_view_atomic [simp]:
-  "view_atomic K (full_view o K)"
-  by (simp add: view_atomic_def)
-
-lemma full_view_wellformed:
-  assumes "\<And>k. K k \<noteq> []"
-  shows "view_wellformed K (full_view o K)"
-  using assms
-  by (auto simp add: view_wellformed_defs kvs_initialized_def zero_in_full_view)
-
-\<comment> \<open>view lemmas\<close>
-lemma view_order_transitive:
-  "u \<sqsubseteq> u' \<Longrightarrow> u' \<sqsubseteq> u'' \<Longrightarrow> u \<sqsubseteq> u''"
-  by (auto simp add: view_order_def)
-
-lemma view_order_refl [simp]:
-  "u \<sqsubseteq> u" by (simp add: view_order_def)
-
-lemma view_order_full_view_increasing:
-  assumes "\<And>k. length (K k) \<le> length (K' k)"
-  shows "(\<lambda>k. full_view (K k)) \<sqsubseteq> (\<lambda>k. full_view (K' k))"
-  using assms
-  by (simp add: full_view_def view_order_def)
 
 lemma view_finite [simp]:
   assumes "view_in_range K u"
@@ -378,46 +429,118 @@ lemma view_zero_full_view:
   using assms
   by (auto simp add: view_in_range_defs)
 
-lemma max_in_full_view [simp]:
-  assumes "vl \<noteq> []"
-  shows "Max (full_view vl) \<in> full_view vl"
-  using assms
-  by (metis full_view_def key_view_Max_full_view key_view_in_range_def
-      length_greater_0_conv lessThan_iff set_eq_subset)
 
-\<comment> \<open>Order lemmas\<close>
+text \<open>Atomic views\<close>
+
+definition view_atomic :: "('v, 'm) kvs_store \<Rightarrow> view \<Rightarrow> bool" where
+  "view_atomic K u \<longleftrightarrow> (\<forall>k k'. \<forall>i \<in> u k. \<forall>i' \<in> full_view (K k').
+      v_writer (K k!i) = v_writer (K k'!i') \<longrightarrow> i' \<in> u k')"
+
+lemmas view_atomicI = view_atomic_def [THEN iffD2, rule_format]
+lemmas view_atomicE [elim] = view_atomic_def [THEN iffD1, elim_format, rule_format]
+
+lemma view_atomic_full_view [simp]: "view_atomic K (full_view o K)"
+  by (simp add: view_atomic_def)
+
+
+
+
+
+
+text \<open>View well-formedness\<close>
+
+definition view_wellformed :: "('v, 'm) kvs_store \<Rightarrow> view \<Rightarrow> bool" where
+  "view_wellformed K u \<longleftrightarrow> view_in_range K u \<and> view_atomic K u"
+
+lemmas view_wellformedD1 [dest] = view_wellformed_def [THEN iffD1, THEN conjunct1]
+lemmas view_wellformedD2 [dest] = view_wellformed_def [THEN iffD1, THEN conjunct2]
+
+lemmas view_wellformed_defs = 
+  view_wellformed_def view_in_range_defs view_atomic_def 
+
+lemma full_view_wellformed:
+  assumes "\<And>k. K k \<noteq> []"
+  shows "view_wellformed K (full_view o K)"
+  using assms
+  by (auto simp add: view_wellformed_defs kvs_initialized_def)
+
+
+subsubsection \<open>Version and KVS orders\<close>
+
+text \<open>Version order\<close>
 
 definition version_order :: "('v, 'm) version_scheme \<Rightarrow> ('v, 'm) version_scheme \<Rightarrow> bool" (infix "\<sqsubseteq>\<^sub>v\<^sub>e\<^sub>r" 60) where
-  "v1 \<sqsubseteq>\<^sub>v\<^sub>e\<^sub>r v2 \<equiv>
+  "v1 \<sqsubseteq>\<^sub>v\<^sub>e\<^sub>r v2 \<longleftrightarrow>
     v_value v1 = v_value v2 \<and>
     v_writer v1 = v_writer v2 \<and>
     v_readerset v1 \<subseteq> v_readerset v2"
 
-lemma version_order_refl [simp]: "v \<sqsubseteq>\<^sub>v\<^sub>e\<^sub>r v" by (simp add: version_order_def)
+lemma version_order_refl [simp]: "v \<sqsubseteq>\<^sub>v\<^sub>e\<^sub>r v" 
+  by (simp add: version_order_def)
+
 lemma version_order_trans: "v1 \<sqsubseteq>\<^sub>v\<^sub>e\<^sub>r v2 \<Longrightarrow> v2 \<sqsubseteq>\<^sub>v\<^sub>e\<^sub>r v3 \<Longrightarrow> v1 \<sqsubseteq>\<^sub>v\<^sub>e\<^sub>r v3"
   by (auto simp add: version_order_def)
 
-definition vlist_order :: "('v, 'm) vs_list \<Rightarrow> ('v, 'm) vs_list \<Rightarrow> bool" (infix "\<sqsubseteq>\<^sub>v\<^sub>l" 60) where
-  "vl1 \<sqsubseteq>\<^sub>v\<^sub>l vl2 \<equiv> length vl1 \<le> length vl2 \<and> (\<forall>i \<in> full_view vl1. vl1!i \<sqsubseteq>\<^sub>v\<^sub>e\<^sub>r vl2!i)"
 
-lemma vlist_order_refl [simp]: "vl \<sqsubseteq>\<^sub>v\<^sub>l vl" by (simp add: vlist_order_def)
-lemma vlist_order_trans: "vl1 \<sqsubseteq>\<^sub>v\<^sub>l vl2 \<Longrightarrow> vl2 \<sqsubseteq>\<^sub>v\<^sub>l vl3 \<Longrightarrow> vl1 \<sqsubseteq>\<^sub>v\<^sub>l vl3"
-  apply (simp add: vlist_order_def) using full_view_length_increasing version_order_trans by blast
+text \<open>Version list order\<close>
+
+definition vlist_order :: "('v, 'm) vs_list \<Rightarrow> ('v, 'm) vs_list \<Rightarrow> bool" (infix "\<sqsubseteq>\<^sub>v\<^sub>l" 60) where
+  "vl1 \<sqsubseteq>\<^sub>v\<^sub>l vl2 \<longleftrightarrow> full_view vl1 \<subseteq> full_view vl2 \<and> (\<forall>i \<in> full_view vl1. vl1!i \<sqsubseteq>\<^sub>v\<^sub>e\<^sub>r vl2!i)"
+
+lemma vlist_order_refl [simp]: "vl \<sqsubseteq>\<^sub>v\<^sub>l vl" 
+  by (simp add: vlist_order_def)
+
+lemma vlist_order_trans: "\<lbrakk> vl1 \<sqsubseteq>\<^sub>v\<^sub>l vl2; vl2 \<sqsubseteq>\<^sub>v\<^sub>l vl3 \<rbrakk> \<Longrightarrow> vl1 \<sqsubseteq>\<^sub>v\<^sub>l vl3"
+  by (meson dual_order.trans in_mono version_order_trans vlist_order_def)
+
+
+text \<open>KVS order\<close>
 
 definition kvs_expands :: "('v, 'm) kvs_store \<Rightarrow> ('v, 'm) kvs_store \<Rightarrow> bool" (infix "\<sqsubseteq>\<^sub>k\<^sub>v\<^sub>s" 60) where
-  "K1 \<sqsubseteq>\<^sub>k\<^sub>v\<^sub>s K2 \<equiv> (\<forall>k. (K1 k) \<sqsubseteq>\<^sub>v\<^sub>l (K2 k)) \<and> view_atomic K2 (\<lambda>k. full_view (K1 k))"
+  "K1 \<sqsubseteq>\<^sub>k\<^sub>v\<^sub>s K2 \<longleftrightarrow> (\<forall>k. (K1 k) \<sqsubseteq>\<^sub>v\<^sub>l (K2 k)) \<and> view_atomic K2 (full_view o K1)"
 
-lemma kvs_exnpands_length_increasing:
+lemmas kvs_expandsI = 
+  kvs_expands_def[THEN iffD2, OF conjI]  (* why isn't rule_format doing this?*)
+
+lemma kvs_expandsE [elim]: 
+  "\<lbrakk> K1 \<sqsubseteq>\<^sub>k\<^sub>v\<^sub>s K2; 
+     \<lbrakk> \<And>k. (K1 k) \<sqsubseteq>\<^sub>v\<^sub>l (K2 k); view_atomic K2 (full_view o K1) \<rbrakk> \<Longrightarrow> P \<rbrakk> 
+   \<Longrightarrow> P"
+  by (simp add: kvs_expands_def)
+
+
+lemma kvs_expands_refl [simp]: "K \<sqsubseteq>\<^sub>k\<^sub>v\<^sub>s K"
+  by (simp add: kvs_expands_def)
+
+lemmas view_atomicD = view_atomic_def [THEN iffD1, rule_format, unfolded view_atomic_def]
+
+
+lemma kvs_expands_trans: 
+  assumes "K1 \<sqsubseteq>\<^sub>k\<^sub>v\<^sub>s K2" and "K2 \<sqsubseteq>\<^sub>k\<^sub>v\<^sub>s K3"
+  shows "K1 \<sqsubseteq>\<^sub>k\<^sub>v\<^sub>s K3"
+  using assms
+proof (intro kvs_expandsI allI)
+  show "view_atomic K3 (full_view \<circ> K1)" using assms
+    by (intro view_atomicI)     (* MAYBE PROVE LEMMAS ABOUT view_atomic? *)
+       (smt (verit) comp_def full_view_length_increasing full_view_subset_is_length_leq 
+            kvs_expands_def version_order_def view_atomic_def vlist_order_def)
+qed (auto intro: vlist_order_trans)
+
+
+(*
+lemma kvs_expands_length_increasing:
   "K1 \<sqsubseteq>\<^sub>k\<^sub>v\<^sub>s K2 \<Longrightarrow> length (K1 k) \<le> length (K2 k)"
   by (simp add: kvs_expands_def vlist_order_def)
 
-lemma kvs_exnpands_still_in_full_view:
+lemma kvs_expands_still_in_full_view:
   "K1 \<sqsubseteq>\<^sub>k\<^sub>v\<^sub>s K2 \<Longrightarrow> i \<in> full_view (K1 k) \<Longrightarrow> i \<in> full_view (K2 k)"
-  using full_view_length_increasing kvs_exnpands_length_increasing by blast
+  using full_view_length_increasing kvs_expands_length_increasing by blast
+*)
+
+
 
 lemma kvs_expanded_view_wellformed:
-  assumes "view_wellformed K1 u"
-    and "K1 \<sqsubseteq>\<^sub>k\<^sub>v\<^sub>s K2"
+  assumes "view_wellformed K1 u" and "K1 \<sqsubseteq>\<^sub>k\<^sub>v\<^sub>s K2"
   shows "view_wellformed K2 u"
   using assms
   apply (auto simp add: view_wellformed_defs kvs_expands_def vlist_order_def full_view_def)
@@ -425,28 +548,15 @@ lemma kvs_expanded_view_wellformed:
   unfolding lessThan_def version_order_def
   subgoal for k k' i i' apply (cases "i' < length (K1 k')")
   apply (metis (no_types, lifting) in_mono mem_Collect_eq)
-    by (metis (no_types, lifting) mem_Collect_eq subset_iff).
+    by (metis (no_types, lifting) mem_Collect_eq subset_iff)
+  done
 
-lemma view_is_atomic:
-  assumes "\<forall>k k'. \<forall>i\<in>full_view (K1 k). \<forall>i'\<in>full_view (K2 k').
-    v_writer (K2 k ! i) = v_writer (K2 k' ! i') \<longrightarrow> i' \<in> full_view (K1 k')"
-    and "i \<in> full_view (K1 k)"
-    and "i' \<in> full_view (K2 k')"
-    and "v_writer (K2 k ! i) = v_writer (K2 k' ! i')"
-  shows "i' \<in> full_view (K1 k')"
-  using assms
-  by simp
 
-lemma kvs_expands_refl [simp]: "K \<sqsubseteq>\<^sub>k\<^sub>v\<^sub>s K" by (simp add: kvs_expands_def view_atomic_def)
-lemma kvs_expands_trans: "K1 \<sqsubseteq>\<^sub>k\<^sub>v\<^sub>s K2 \<Longrightarrow> K2 \<sqsubseteq>\<^sub>k\<^sub>v\<^sub>s K3 \<Longrightarrow> K1 \<sqsubseteq>\<^sub>k\<^sub>v\<^sub>s K3"
-  apply (auto simp add: kvs_expands_def view_atomic_def)
-  using vlist_order_trans apply blast
-  subgoal for k k' i i'   
-    apply (auto dest!: view_is_atomic[of K1 K2 i k i' k'])
-    apply (auto dest!: view_is_atomic[of K2 K3 i k i' k'])
-    using full_view_length_increasing vlist_order_def apply blast
-    using full_view_length_increasing vlist_order_def apply blast
-    by (metis (no_types) full_view_length_increasing version_order_def vlist_order_def).
+
+
+
+(************)
+(************)
 
 
 \<comment> \<open>List updates and membership lemmas\<close>
@@ -528,34 +638,39 @@ lemma longer_list_not_empty:
   by auto
 
 
-subsection \<open>Snapshots and Configs\<close>
+(************)
+(************)
+
+
+
+
+
+
+
+subsection \<open>Snapshots\<close>
 
 type_synonym 'v snapshot = "key \<Rightarrow> 'v"
 
-definition last_version :: "('v, 'm) vs_list \<Rightarrow> key_view \<Rightarrow> ('v, 'm) version_scheme" where
+(* REMOVE last_version? *)
+
+abbreviation last_version :: "('v, 'm) vs_list \<Rightarrow> key_view \<Rightarrow> ('v, 'm) version_scheme" where
   "last_version vl uk \<equiv> vl ! Max uk"
 
 definition view_snapshot :: "('v, 'm) kvs_store \<Rightarrow> view \<Rightarrow> 'v snapshot" where
   "view_snapshot K u k \<equiv> v_value (last_version (K k) (u k))"
 
-type_synonym 'v config = "'v kv_store \<times> (cl_id \<Rightarrow> view)"
 
-abbreviation c_views_init :: "cl_id \<Rightarrow> view" where
-  "c_views_init \<equiv> (\<lambda>cl. view_init)"
-
-definition config_init :: "'v config" where
-  "config_init \<equiv> (kvs_init, c_views_init)"
-
-lemmas config_init_defs = config_init_def (* kvs_init_defs *) view_init_def
 
 \<comment> \<open>Lemmas about last_version\<close>
 
-lemma [simp]: "last_version [v] {..<Suc 0} = v"        (* CHSP: seems very specialized *)
-  by (auto simp add: last_version_def lessThan_def)
+lemma [simp]: "last_version [v] {..<Suc 0} = v"   (* REMOVE *) (* CHSP: seems very specialized *)
+  by (auto simp add: lessThan_def)
 
-lemma Max_less_than_Suc [simp]: "Max {..<Suc n} = n" 
+lemma Max_less_than_Suc [simp]: "Max {..<Suc n} = n"    (* REMOVE *)
   apply (simp add: lessThan_Suc)
   by (meson Max_insert2 finite_lessThan lessThan_iff less_imp_le_nat)
+
+
 
 
 subsection \<open>Fingerprints\<close>
@@ -617,246 +732,293 @@ definition fp_property :: "'v fingerpr \<Rightarrow> ('v, 'm) kvs_store \<Righta
   "fp_property F K u \<equiv> \<forall>k. R \<in> dom (F k) \<longrightarrow> F k R = Some (view_snapshot K u k)"
 
 
-
 subsection \<open>KVS updates\<close>
 
-definition update_kv_key_reads :: 
-  "txid0 \<Rightarrow> 'v key_fp \<Rightarrow> key_view \<Rightarrow> ('v, 'm) vs_list \<Rightarrow> ('v, 'm) vs_list" where
-  "update_kv_key_reads t Fk uk vl =
-    (case Fk R of
-      None   \<Rightarrow> vl |
-      Some v \<Rightarrow> let lv = last_version vl uk in
-                vl[Max uk := lv\<lparr>v_readerset := insert t (v_readerset lv)\<rparr>])"
+fun update_kv_key_reads :: "txid0 \<Rightarrow> 'v option \<Rightarrow> key_view \<Rightarrow> ('v, 'm) vs_list \<Rightarrow> ('v, 'm) vs_list" where
+  "update_kv_key_reads t None uk vl = vl" |
+  "update_kv_key_reads t (Some _) uk vl = 
+     (let lv = last_version vl uk in vl[Max uk := lv\<lparr>v_readerset := insert t (v_readerset lv)\<rparr>])"
 
-definition update_kv_key_writes :: "txid0 \<Rightarrow> 'v key_fp \<Rightarrow> 'v v_list \<Rightarrow> 'v v_list" where
-  "update_kv_key_writes t Fk vl =
-    (case Fk W of
-      None   \<Rightarrow> vl |
-      Some v \<Rightarrow> vl @ [new_vers (Tn t) v])"
+fun update_kv_key_writes :: "txid0 \<Rightarrow> 'v option \<Rightarrow> 'v v_list \<Rightarrow> 'v v_list" where
+  "update_kv_key_writes t None vl = vl" |
+  "update_kv_key_writes t (Some v) vl = vl @ [new_vers (Tn t) v]"
 
 definition update_kv_key :: "txid0 \<Rightarrow> 'v key_fp \<Rightarrow> key_view \<Rightarrow> 'v v_list \<Rightarrow> 'v v_list" where
-  "update_kv_key t Fk uk = (update_kv_key_writes t Fk) o (update_kv_key_reads t Fk uk)"
+  "update_kv_key t Fk uk = update_kv_key_writes t (Fk W) o update_kv_key_reads t (Fk R) uk"
 
 definition update_kv :: "txid0 \<Rightarrow> 'v fingerpr \<Rightarrow> view \<Rightarrow> 'v kv_store \<Rightarrow> 'v kv_store" where
   "update_kv t F u K = (\<lambda>k. update_kv_key t (F k) (u k) (K k))"
 
-lemmas update_kv_key_reads_defs = update_kv_key_reads_def Let_def last_version_def
-
+(*
+lemmas update_kv_key_reads_defs = Let_def
+*)
 lemmas update_kv_defs = update_kv_def update_kv_key_def
 
 
-subsubsection \<open>Version list updates\<close>
+subsubsection \<open>Lemmas about length of updates\<close>
 
-lemma update_kv_key_reads_read_latest:
-  assumes "Fk R = Some v" "Max uk < length vl"
-  shows "update_kv_key_reads t Fk uk vl ! Max uk = 
-         (last_version vl uk)\<lparr>v_readerset := insert t (v_readerset (last_version vl uk))\<rparr>"
-  using assms
-  by (simp add: update_kv_key_reads_def Let_def split: op_type.split)
-
-lemma update_kv_key_reads_read_not_latest:
-  assumes "Fk R = Some v" "i \<noteq> Max uk"
-  shows "update_kv_key_reads t Fk uk vl ! i = vl ! i"
-  using assms
-  by (simp add: update_kv_key_reads_def Let_def split: op_type.split)
-
-lemma update_kv_key_reads_no_read:
-  assumes "Fk R = None"
-  shows "update_kv_key_reads t Fk uk vl = vl"
-  using assms
-  by (simp add: update_kv_key_reads_def split: op_type.split)
-
-lemmas update_kv_key_reads_simps = 
-   update_kv_key_reads_read_latest update_kv_key_reads_read_not_latest update_kv_key_reads_no_read
-
-
-(*
-lemma update_kv_key_writes:
-  "update_kv_key_writes t Fk vl = 
-   (case Fk W of None \<Rightarrow> vl | Some v \<Rightarrow> vl @ [new_vers t v])"
-  by (auto simp add: update_kv_key_writes_def)
-
-lemmas update_kv_key_writes_simps = update_kv_key_writes
-*)
-
-lemma update_kv_key_write_only:
-  "update_kv_key t (case_op_type None wo) uk vl = 
-   (case wo of None \<Rightarrow> vl | Some v \<Rightarrow> vl @ [new_vers (Tn t) v])"
-   by (auto simp add: update_kv_key_def update_kv_key_reads_simps update_kv_key_writes_def)
-
-
-
-
-(* next one is about KVS update: *)
-
-lemma update_kv_write_only:
-  "update_kv t (write_only_fp kv_map) u K k = 
-   (case kv_map k of None \<Rightarrow> K k | Some v \<Rightarrow> K k @ [new_vers (Tn t) v])"
-  by (simp add: update_kv_def write_only_fp_def update_kv_key_write_only)
-
-
-
-
-
-
-
-
-
-
-
-
-lemma update_kv_key_empty_fp [simp]:
-  assumes "Fk R = None" and "Fk W = None"
-  shows "update_kv_key t Fk uk vl = vl"
-  using assms
-  by (auto simp add: update_kv_key_def update_kv_key_reads_def update_kv_key_writes_def)
-
-
-(* next two are about views *)
-
-lemma update_kv_key_ro_full_view [simp]:
-  assumes "Fk W = None"
-  shows "full_view (update_kv_key t Fk uk vl) = full_view vl"
-  using assms
-  by (auto simp add: update_kv_key_def update_kv_key_writes_def update_kv_key_reads_defs
-       split: option.split)
-
-lemma update_kv_key_rw_full_view [simp]:
-  assumes "Fk W \<noteq> None"
-  shows "full_view (update_kv_key t Fk uk vl) = insert (length vl) (full_view vl)"
-  using assms
-  by (auto simp add: update_kv_key_def update_kv_key_writes_def update_kv_key_reads_defs
-      full_view_grows length_vl_in_appended split: option.split)
-
-
-
-lemma update_kv_key_ro_set_v_readerset:
-  assumes "Fk W = None"
-    and "vl \<noteq> []"
-  shows "(update_kv_key t Fk (full_view vl) vl) [Max (full_view vl) :=
-    last_version (update_kv_key t Fk (full_view vl) vl) (full_view vl) \<lparr> v_readerset := x \<rparr>] =
-    vl [Max (full_view vl) := last_version vl (full_view vl) \<lparr> v_readerset := x \<rparr>]"
-  using assms
-  by (auto simp add: update_kv_key_def update_kv_key_writes_def update_kv_key_reads_defs
-      split: option.split)
-
-lemma update_kv_key_ro_v_readerset [simp]:
-  assumes "Fk W = None" and "Fk R \<noteq> None"
-    and "vl \<noteq> []"
-  shows "v_readerset (last_version (update_kv_key t Fk (full_view vl) vl) (full_view vl)) =
-         insert t (v_readerset (last_version vl (full_view vl)))"
-  using assms
-  by (auto simp add: update_kv_key_def update_kv_key_writes_def update_kv_key_reads_defs)
-
-
-
-
-subsubsection \<open>Lemmas about length of version list updates\<close>
-
-\<comment> \<open>update_kv lemmas about version list length and full_view\<close>
-
-lemma update_kv_key_reads_length:
-  "length (update_kv_key_reads t Fk uk vl) = length vl"
-proof (cases "Fk R")
-  case (Some a)
-  then show ?thesis apply (auto simp add: update_kv_key_reads_def)
-    by (meson length_list_update)
-qed (auto simp add: update_kv_key_reads_def)
-
-lemma update_kv_key_writes_none_length:
-  assumes "Fk W = None"
-  shows "length (update_kv_key_writes t Fk vl) = length vl"
-  using assms by (auto simp add: update_kv_key_writes_def)
-
-lemma update_kv_key_writes_some_length:
-  assumes "Fk W = Some v"
-  shows "length (update_kv_key_writes t Fk vl) = Suc (length vl)"
-  using assms by (auto simp add: update_kv_key_writes_def)
+lemma update_kv_key_reads_length [simp]:
+  "length (update_kv_key_reads t vo uk vl) = length vl"
+  by (cases vo) (simp_all add: Let_def)
 
 lemma update_kv_key_writes_length:
-  shows "length (update_kv_key_writes t Fk vl) = Suc (length vl) \<or> 
-         length (update_kv_key_writes t Fk vl) = length vl"
-  by (cases "Fk W") (auto simp add: update_kv_key_writes_def)
+  "length (update_kv_key_writes t vo vl) = (if vo = None then length vl else Suc (length vl))"
+  by (auto)
 
-lemma update_kv_key_writes_length_increasing:
+lemma update_kv_key_length:
+  "length (update_kv_key t Fk uk vl) = (if Fk W = None then length vl else Suc (length vl))"
+  by (simp add: update_kv_key_def update_kv_key_writes_length)
+
+lemma update_kv_key_writes_length_increasing [intro!]:    (* AUT-ADDED *)
   "length vl \<le> length (update_kv_key_writes t Fk vl)"
-  using update_kv_key_writes_length [of t Fk vl]
-  by auto
+  by (simp add: update_kv_key_writes_length)
+
+(* REMOVE?
+lemma update_kv_key_writes_length:
+  "length (update_kv_key_writes t vo vl) = Suc (length vl) \<or> 
+   length (update_kv_key_writes t vo vl) = length vl"
+  by (auto simp add: update_kv_key_writes_length)
+*)
+
+lemma update_kv_key_length_increasing [intro!]:        (* AUT-ADDED *)
+  "length vl \<le> length (update_kv_key t Fk uk vl)"
+  by (simp add: update_kv_key_length)
 
 lemma update_kv_key_writes_on_diff_len:
   assumes "length vl1 \<le> length vl2"
   shows "length (update_kv_key_writes t Fk vl1) \<le>
          length (update_kv_key_writes t Fk vl2)"
-  using assms by (auto simp add: update_kv_key_writes_def split: option.split)
+  using assms 
+  by (auto simp add: update_kv_key_writes_length)
 
+(* REMOVE?
 lemma update_kv_key_length:
   "length (update_kv_key t Fk uk vl) = Suc (length vl) \<or>
    length (update_kv_key t Fk uk vl) = length vl"
-  using update_kv_key_writes_length [where vl="update_kv_key_reads t Fk uk vl"]
-  by (simp add: update_kv_defs update_kv_key_reads_length)
+  by (simp add: update_kv_key_length)
+*)
 
-lemma update_kv_key_length_increasing:
-  "length vl \<le> length (update_kv_key t Fk uk vl)"
-  using update_kv_key_length [of t Fk uk vl]
-  by auto
 
+lemma update_kv_length:
+  "length (update_kv t F u K k) = (if F k W = None then length (K k) else Suc (length (K k)))"
+  by (simp add: update_kv_def update_kv_key_length)
+
+lemmas length_update_kv = update_kv_length  (* eventually remove one name... *)
+
+lemma update_kv_length_increasing [intro!]:        (* AUT-ADDED *)      
+  "length (K k) \<le> length (update_kv t F u K k)"
+  by (simp add: update_kv_length)
+
+(* REMOVE?
 lemma update_kv_length:
   "length (update_kv t F u K k) = Suc (length (K k)) \<or>
    length (update_kv t F u K k) = length (K k)"
   by (simp add: update_kv_def update_kv_key_length)
- 
-lemma update_kv_length_increasing:      
-  "length (K k) \<le> length (update_kv t F u K k)"
-  using update_kv_length [of t F u K k]
-  by auto
+*)
 
 
-
-subsubsection \<open>Lemmas about full view\<close>
-
+subsubsection \<open>Lemmas about full view of updates\<close>
 
 lemma full_view_update_kv_key_reads [simp]:
   "full_view (update_kv_key_reads t Fk uk vl) = full_view vl"
-  by (simp add: update_kv_key_reads_length full_view_def)
+  by (simp)
 
 lemma full_view_update_kv_key_writes [dest]:
   "i \<in> full_view vl \<Longrightarrow> i \<in> full_view (update_kv_key_writes t Fk vl)"
   using update_kv_key_writes_length_increasing [of vl t Fk] 
   by (simp add: full_view_def)
 
-lemma full_view_update_kv [dest]:
+lemma full_view_update_kv_incl [dest]:
   "i \<in> full_view (K k) \<Longrightarrow> i \<in> full_view (update_kv t F u K k)"
   using update_kv_length_increasing [of K k t F u] 
   by (simp add: full_view_def)
 
+
+lemma update_kv_key_ro_full_view [simp]:     (* remove from simp set? *)
+  assumes "Fk W = None"
+  shows "full_view (update_kv_key t Fk uk vl) = full_view vl"
+  using assms
+  by (simp add: update_kv_key_length)
+
+lemma update_kv_key_rw_full_view [simp]:     (* remove from simp set? *)
+  assumes "Fk W \<noteq> None"
+  shows "full_view (update_kv_key t Fk uk vl) = insert (length vl) (full_view vl)"
+  using assms
+  by (auto simp add: update_kv_key_def)
+
+lemma full_view_update_kv:                   (* add to simp set? NO. *)
+  "full_view (update_kv t F u K k) = 
+   (if F k W = None then full_view (K k) else insert (length (K k)) (full_view (K k)))"
+  by (simp add: update_kv_def)
+
+
+(* REMOVE?
 lemma not_full_view_update_kv:
   assumes "i \<in> full_view (update_kv t F u K k)" and "i \<notin> full_view (K k)"
   shows "i = length (K k) \<and> length (update_kv t F u K k) = Suc (length (K k))"
   using assms update_kv_length [of t F u K k]
   by (auto simp add: less_Suc_eq_le full_view_def)
+*)
 
+(* REMOVE?
 lemma update_kv_key_writes_key_decides_length:
-  shows "length (update_kv_key t Fk uk vl) = length (update_kv_key_writes t Fk vl)"
-  by (cases "Fk W") (auto simp add: update_kv_key_def update_kv_key_writes_def update_kv_key_reads_length)
+  shows "length (update_kv_key t Fk uk vl) = length (update_kv_key_writes t (Fk W) vl)"
+  by (cases "Fk W") (auto simp add: update_kv_key_def update_kv_key_reads_length)
 
 lemma update_kv_key_writes_decides_length:
-  shows "length (update_kv t F u K k) = length (update_kv_key_writes t (F k) (K k))"
+  shows "length (update_kv t F u K k) = length (update_kv_key_writes t (F k W) (K k))"
   by (simp add: update_kv_def update_kv_key_writes_key_decides_length)
+*)
 
 
 
+subsubsection \<open>Accessing updated version lists\<close>
 
-\<comment> \<open>update_kv lemmas about changing the versions\<close>
+text \<open>Reads\<close>
 
-lemma update_kv_key_writes_version_inv:
-  assumes "i \<in> full_view vl"
-  shows "update_kv_key_writes t Fk vl!i = vl!i"
-proof (cases "Fk W")
-  case (Some a)
-  then show ?thesis using assms
-    by (auto simp add: update_kv_key_writes_def)
-qed (auto simp add: update_kv_key_writes_def)
+lemma update_kv_key_reads_not_latest:
+  assumes "i \<noteq> Max uk"
+  shows "update_kv_key_reads t vo uk vl!i = vl!i"
+  using assms
+  by  (cases vo) (simp_all add: Let_def)
 
+lemma update_kv_key_reads_latest:
+  assumes "i = Max uk" "i \<in> full_view vl" "vo = Some v"
+  shows "update_kv_key_reads t vo uk vl!i = (vl!i)\<lparr>v_readerset := insert t (v_readerset (vl!i))\<rparr>"
+  using assms
+  by (simp add: Let_def)
+
+text \<open>Note: case of no read, @{prop "vo = None"} goes by simp.\<close>
+
+lemmas update_kv_key_reads_simps = 
+   update_kv_key_reads_latest update_kv_key_reads_not_latest 
+
+
+text \<open>Writes\<close>
+
+lemma update_kv_key_writes_old:
+  assumes "i \<in> full_view vl" 
+  shows "update_kv_key_writes t vo vl!i = vl!i"
+  using assms
+  by (cases vo) auto
+
+text \<open>Note: cases of no write and accessing last write go by simp.\<close>
+
+(* redundant, goes by simp
+
+lemma update_kv_key_writes_new:
+  assumes "i = length vl" "vo = Some v" 
+  shows "update_kv_key_writes t vo vl!i = new_vers (Tn t) v"
+  using assms
+  by simp
+*)
+
+lemmas update_kv_key_writes_simps = update_kv_key_writes_old
+
+
+text \<open>Reads and writes\<close>
+
+lemma update_kv_key_nop [simp]:
+  assumes "Fk W = None" "Fk R = None" 
+  shows "update_kv_key t Fk uk vl = vl"
+  using assms
+  by (simp add: update_kv_key_def)
+
+lemma update_kv_key_write_only:
+  "update_kv_key t (case_op_type None wo) uk vl = 
+   (case wo of None \<Rightarrow> vl | Some v \<Rightarrow> vl @ [new_vers (Tn t) v])"
+   by (auto simp add: update_kv_key_def split: option.split)
+
+lemma update_kv_key_old_no_read:
+  assumes "i \<in> full_view vl" "Fk R = None" 
+  shows "update_kv_key t Fk uk vl!i = vl!i"
+  using assms
+  by (simp add: update_kv_key_def update_kv_key_writes_simps)
+
+lemma update_kv_key_old_not_latest:
+  assumes "i \<in> full_view vl" "i \<noteq> Max uk"
+  shows "update_kv_key t Fk uk vl!i = vl!i"
+  using assms
+  by (simp add: update_kv_key_def update_kv_key_writes_simps update_kv_key_reads_simps)
+
+lemma update_kv_key_old_latest:
+  assumes "i \<in> full_view vl" "i = Max uk" "Fk R = Some v" 
+  shows "update_kv_key t Fk uk vl!i = (vl!i)\<lparr>v_readerset := insert t (v_readerset (vl!i))\<rparr>"
+  using assms
+  by (simp add: update_kv_key_def Let_def update_kv_key_writes_simps)
+
+lemma update_kv_key_new:
+  assumes "i = length vl" "Fk W = Some v" 
+  shows "update_kv_key t Fk uk vl!i = new_vers (Tn t) v"
+  using assms
+  by (simp add: update_kv_key_def update_kv_key_writes_simps update_kv_key_reads_simps 
+                nth_append_length')
+
+lemmas update_kv_key_simps = 
+  update_kv_key_old_no_read update_kv_key_old_latest update_kv_key_old_not_latest update_kv_key_new
+
+
+text \<open>KVS\<close>
+
+lemma update_kv_empty:
+  "update_kv t F u K k = [] \<Longrightarrow> K k = []"
+  using length_update_kv[of t F u K k]
+  by (simp split: if_split_asm)
+
+lemma update_kv_old_nop [simp]:
+  assumes "F k W = None" "F k R = None"
+  shows "update_kv t F u K k = K k"
+  using assms
+  by (simp add: update_kv_def update_kv_key_simps)
+
+lemma update_kv_write_only:
+  "update_kv t (write_only_fp kv_map) u K k = 
+   (case kv_map k of None \<Rightarrow> K k | Some v \<Rightarrow> K k @ [new_vers (Tn t) v])"
+  by (simp add: update_kv_def write_only_fp_def update_kv_key_write_only)
+
+lemma update_kv_old_no_read:
+  assumes "i \<in> full_view (K k)" "F k R = None"
+  shows "update_kv t F u K k!i = K k!i"
+  using assms
+  by (simp add: update_kv_def update_kv_key_simps)
+
+lemma update_kv_old_not_latest:
+  assumes "i \<in> full_view (K k)" "i \<noteq> Max (u k)"
+  shows "update_kv t F u K k!i = K k!i"
+  using assms
+  by (simp add: update_kv_def update_kv_key_simps)
+
+lemma update_kv_old_latest:
+  assumes "i \<in> full_view (K k)" "i = Max (u k)" "F k R = Some v"
+  shows "update_kv t F u K k!i = (K k!i)\<lparr>v_readerset := insert t (v_readerset (K k!i))\<rparr>"
+  using assms
+  by (simp add: update_kv_def update_kv_key_simps)
+
+lemma update_kv_new:
+  assumes "i = length (K k)" "F k W = Some v"
+  shows "update_kv t F u K k!i = new_vers (Tn t) v"
+  using assms
+  by (simp add: update_kv_def update_kv_key_simps)
+
+lemmas update_kv_simps =
+  update_kv_old_no_read update_kv_old_not_latest update_kv_old_latest update_kv_new
+
+
+(*******************************)
+(* TODO: integrate stuff below *)
+(*******************************)
+
+lemma "vl \<noteq> [] \<Longrightarrow> Max (full_view vl) \<in> full_view vl"
+  apply (auto simp add: full_view_def)
+  oops
+
+lemma update_kv_key_ro_set_v_readerset:
+  assumes "Fk W = None" and "vl \<noteq> []"
+  shows "(update_kv_key t Fk (full_view vl) vl) [Max (full_view vl) :=
+    last_version (update_kv_key t Fk (full_view vl) vl) (full_view vl) \<lparr> v_readerset := x \<rparr>] =
+    vl [Max (full_view vl) := last_version vl (full_view vl) \<lparr> v_readerset := x \<rparr>]"
+  using assms
+  by (cases "Fk R") (simp_all add: update_kv_key_def Let_def)
 
 
 
@@ -865,46 +1027,50 @@ subsubsection \<open>Lemmas about version value\<close>
 (* v_value *)
 lemma update_kv_key_reads_v_value_inv:
   assumes "i \<in> full_view vl"
-  shows "v_value (update_kv_key_reads t Fk uk vl!i) = v_value (vl!i)"
-proof (cases "Fk R")
-  case (Some a)
-  then show ?thesis using assms
-    by (cases "i = Max uk") 
-       (auto simp add: update_kv_key_reads_defs)
-qed (auto simp add: update_kv_key_reads_def)
+  shows "v_value (update_kv_key_reads t vo uk vl ! i) = v_value (vl ! i)"
+  using assms
+  by (cases vo) (simp_all add: Let_def)
 
 lemma update_kv_key_v_value_inv:
   assumes "i \<in> full_view vl"
-  shows "v_value (update_kv_key t Fk uk vl !i) = v_value (vl !i)"
+  shows "v_value (update_kv_key t Fk uk vl ! i) = v_value (vl ! i)"
   using assms
-  by (auto simp add: update_kv_key_def update_kv_key_writes_version_inv update_kv_key_reads_v_value_inv)
+  by (auto simp add: update_kv_key_def update_kv_key_writes_simps update_kv_key_reads_v_value_inv)
 
 lemma update_kv_v_value_inv:
   assumes "i \<in> full_view (K k)"
-  shows "v_value (update_kv t F u K k!i) = v_value (K k!i)"
+  shows "v_value (update_kv t F u K k ! i) = v_value (K k ! i)"
   using assms
   by (auto simp add: update_kv_def update_kv_key_v_value_inv)
 
+lemmas update_kv_v_value_simps = update_kv_v_value_inv
 
 
 subsubsection \<open>Lemmas about version writer\<close>
 
 (* v_writer *)
-lemma update_kv_key_reads_v_writer_inv:
+lemma update_kv_key_reads_v_writer_old:
   assumes "i \<in> full_view vl"
-  shows "v_writer (update_kv_key_reads t Fk uk vl!i) = v_writer (vl!i)"
-proof (cases "Fk R")
-  case (Some a)
-  then show ?thesis using assms
-    by (cases "i = Max uk")
-       (auto simp add: update_kv_key_reads_defs split: option.splits)
-qed (simp add: update_kv_key_reads_def)
+  shows "v_writer (update_kv_key_reads t vo uk vl!i) = v_writer (vl!i)"
+  using assms
+  by (cases vo) (simp_all add: Let_def)
 
-lemma update_kv_v_writer_inv:
+lemma update_kv_v_writer_old: 
   assumes "i \<in> full_view (K k)"
   shows "v_writer (update_kv t F u K k!i) = v_writer (K k!i)"
   using assms
-  by (auto simp add: update_kv_defs update_kv_key_writes_version_inv update_kv_key_reads_v_writer_inv)
+  by (auto simp add: update_kv_defs update_kv_key_writes_simps update_kv_key_reads_v_writer_old)
+
+lemma update_kv_v_writer_new: 
+  assumes "i = length (K k)" "F k W = Some v"
+  shows "v_writer (update_kv t F u K k!i) = Tn t"
+  using assms
+  by (auto simp add: update_kv_simps)
+
+lemmas update_kv_v_writer_simps = 
+  update_kv_v_writer_old update_kv_v_writer_new
+
+(*  REPLACE PREMISES IN LEMMAS BELOW? (with sth about fingerprint)
 
 lemma update_kv_key_writes_key_new_version_v_writer:
   assumes  "length (update_kv_key t Fk uk vl) = Suc (length vl)"
@@ -931,7 +1097,10 @@ lemma update_kv_new_version_v_writer:
   using assms
   apply (auto simp add: update_kv_defs)
   by (metis comp_apply update_kv_key_def update_kv_key_new_version_v_writer)
-            
+*)
+
+
+(*
 lemma update_kv_key_reads_vl_writers_inv [simp]:
   "vl_writers (update_kv_key_reads t Fk uk vl) = vl_writers vl"
   apply (auto simp add: update_kv_key_reads_defs vl_writers_def in_set_conv_nth split: option.split)
@@ -940,47 +1109,154 @@ lemma update_kv_key_reads_vl_writers_inv [simp]:
     apply (metis set_update_memI version.select_convs(2) version.surjective version.update_convs(3))
     by (metis length_list_update nth_list_update_neq nth_mem)
   done
+*)
 
 
 subsubsection \<open>Lemmas about version reader set\<close>
 
-(* v_readerset *)
-lemma v_readerset_update_kv_key_reads_max_u:
-  assumes "x \<in> v_readerset (update_kv_key_reads t Fk uk vl!i)"
+(* SUBSUMED BY NEXT LEMMA
+lemma v_readerset_update_kv_key_reads_max_u':
+  assumes "x \<in> v_readerset (update_kv_key_reads t vo uk vl!i)"
       and "i \<in> full_view vl" and "i = Max uk" 
     shows "x \<in> v_readerset (vl!i) \<or> x = t"
   using assms
-  by (cases "Fk R") (auto simp add: update_kv_key_reads_defs)
+  by (auto simp add: v_readerset_update_kv_key_reads_max_u split: if_split_asm)
+*)
 
-lemma v_readerset_update_kv_key_reads_rest_inv:
+lemma v_readerset_update_kv_key_reads_max_u:
+  assumes "i \<in> full_view vl" and "i = Max uk" 
+  shows "v_readerset (update_kv_key_reads t vo uk vl!i) =
+         (if vo = None then v_readerset (vl!i) else insert t (v_readerset (vl!i)))"
+  using assms
+  by (auto simp add: Let_def)
+
+lemma v_readerset_update_kv_key_reads_not_max:
   assumes "i \<in> full_view vl" and "i \<noteq> Max uk"
-  shows "v_readerset (update_kv_key_reads t Fk uk vl!i) = v_readerset (vl!i)"
-proof (cases "Fk R")
-  case (Some a)
-  then show ?thesis using assms
-    by (auto simp add: update_kv_key_reads_def; metis assms(2) nth_list_update_neq)
-qed (auto simp add: update_kv_key_reads_def)
+  shows "v_readerset (update_kv_key_reads t vo uk vl!i) = v_readerset (vl!i)"
+  using assms
+  by (cases vo) (auto simp add: Let_def)
 
 lemma v_readerset_update_kv_key_writes:
-  assumes "i \<in> full_view vl"
-    shows "v_readerset (update_kv_key_writes t Fk vl ! i) = v_readerset (vl ! i)"
+  assumes "i \<in> full_view vl \<or> vo = None"
+  shows "v_readerset (update_kv_key_writes t vo vl!i) = v_readerset (vl!i)"
   using assms
-  by (auto simp add: update_kv_key_writes_def split: option.splits)
+  by (cases vo) (simp_all)
+
+(* redundant (goes by simp): 
+lemma v_readerset_update_kv_key_writes_new:
+  assumes "i = length vl" "vo = Some v"
+  shows "v_readerset (update_kv_key_writes t vo vl!i) = {}"
+  using assms
+  by (simp)
+*)
+
+lemma v_readerset_update_kv_old:
+  assumes "i \<in> full_view (K k)"
+  shows "v_readerset (update_kv t F u K k ! i) =
+         (if i \<noteq> Max (u k) \<or> F k R = None 
+          then v_readerset (K k!i) else insert t (v_readerset (K k!i)))"
+  using assms
+  by (auto simp add: update_kv_defs v_readerset_update_kv_key_writes 
+                     v_readerset_update_kv_key_reads_not_max Let_def)
+
+lemma v_readerset_update_kv_new:
+  assumes "i = length (K k)" "F k W = Some v"
+  shows "v_readerset (update_kv t F u K k!i) = {}"
+  using assms
+  by (simp add: update_kv_defs nth_append_length')
+
+lemmas v_readerset_update_kv_simps = 
+  v_readerset_update_kv_old v_readerset_update_kv_new
+
+
+(* INTEGRATE TWO LEMMAS BELOW: *)
+
+(* new lemma *)
+lemma v_readerset_update_kv_reads_subset_insert:
+  assumes "i \<in> full_view vl"
+    shows "v_readerset (update_kv_key_reads t vo uk vl!i) \<subseteq> insert t (v_readerset (vl!i))"
+  using assms
+  by (metis subset_insertI update_kv_key_reads_not_latest 
+            v_readerset_update_kv_key_reads_max_u verit_comp_simplify1(2))
+
+(* new lemma *)
+lemma v_readerset_update_kv_reads_subset:
+  assumes "i \<in> full_view vl"
+    shows "v_readerset (vl!i) \<subseteq> v_readerset (update_kv_key_reads t vo uk vl!i)"
+proof (cases vo)
+  case (Some a)
+  then show ?thesis apply (auto simp add: Let_def)
+    by (metis Un_absorb Un_insert_right assms expanding_feature3)
+qed (simp)
+
+
+
+(* new lemma *)
+lemma view_stays_atomic:
+  assumes "t \<in> next_txids K cl"
+  shows "view_atomic (update_kv t F u K) (\<lambda>k. full_view (K k))"
+  using assms
+  apply (simp add: view_atomic_def)
+  by (metis fresh_txid_v_writer full_view_update_kv insertE not_None_eq 
+            update_kv_v_writer_new update_kv_v_writer_old)
+
+(* new lemma *)
+lemma kvs_expands_through_update:
+  assumes "K' = update_kv t F u K"
+    and "t \<in> next_txids K cl"
+  shows "K \<sqsubseteq>\<^sub>k\<^sub>v\<^sub>s K'"
+  using assms
+  apply (auto simp add: kvs_expands_def vlist_order_def update_kv_defs version_order_def
+                        update_kv_key_reads_v_value_inv update_kv_key_reads_v_writer_old 
+                        update_kv_key_writes_simps)
+  apply (metis (no_types, lifting) in_mono v_readerset_update_kv_reads_subset)
+  by (metis (mono_tags, lifting) assms(1) comp_apply view_atomic_def view_stays_atomic)
+
+
+text \<open>Other lemmas: case analyses, ...\<close>
+
+lemma v_readerset_update_kv_old_cases:
+  assumes "t' \<in> v_readerset (update_kv t F u K k ! i)" and "i \<in> full_view (K k)"
+  shows "t' = t \<or> t' \<in> v_readerset (K k!i)"
+  using assms
+  by (simp add: v_readerset_update_kv_old split: if_split_asm)
+
+lemma update_kv_key_ro_v_readerset [simp]:        (* REMOVE from simpset? *)
+  assumes "Fk W = None" and "Fk R = Some v"
+    and "vl \<noteq> []"
+  shows "v_readerset (last_version (update_kv_key t Fk (full_view vl) vl) (full_view vl)) =
+         insert t (v_readerset (last_version vl (full_view vl)))"
+  using assms
+  by (simp add: update_kv_key_def Let_def)
+
+
+lemmas update_kv_version_field_simps = 
+  update_kv_v_value_simps update_kv_v_writer_simps v_readerset_update_kv_simps
+
+
+(* SUBSUMED BY LEMMA v_readerset_update_kv_old_cases (modulo if_split_asm):
 
 lemma v_readerset_update_kv_max_u:
   assumes "x \<in> v_readerset (update_kv t F u K k ! Max (u k))"
       and "view_in_range K u"
     shows "x \<in> v_readerset (K k ! Max (u k)) \<or> x = t"
   using assms
+  by (auto simp add: v_readerset_update_kv split: if_split_asm)
+
   by (auto simp add: update_kv_defs v_readerset_update_kv_key_writes
            dest: v_readerset_update_kv_key_reads_max_u)
+*)
+
+(* REDUNDANT: use update_kv_nth_version
 
 lemma v_readerset_update_kv_rest_inv:
-  assumes "i \<noteq> Max (u k)" and  "i \<in> full_view (K k)"
+  assumes "i \<in> full_view (K k)" and "i \<noteq> Max (u k)" 
   shows "v_readerset (update_kv t F u K k!i) = v_readerset (K k!i)"
-  using assms update_kv_key_writes_version_inv [of i "update_kv_key_reads t (F k) (u k) (K k)"]
-  by (auto simp add: v_readerset_update_kv_key_reads_rest_inv update_kv_defs update_kv_key_reads_length)
+  using assms
+  by (simp add: update_kv_nth_version)
+*)
 
+(* REPLACE BY STH WITH DIFFERENT PREMISES?:
 
 lemma update_kv_key_writes_new_version_v_readerset:
   assumes  "length (update_kv t F u K k) = Suc (length (K k))"
@@ -994,86 +1270,56 @@ lemma update_kv_new_version_v_readerset:
   using assms
   apply (auto simp add: update_kv_defs update_kv_key_writes_def update_kv_key_reads_length split: option.split)
   by (metis update_kv_key_reads_length equals0D nth_append_length version.select_convs(3))
-
-lemma update_kv_key_reads_vl_readers_inv:
-  "vl \<noteq> [] \<Longrightarrow> vl_readers (update_kv_key_reads t Fk (full_view vl) vl) =
-    (case Fk R of None \<Rightarrow> vl_readers vl | Some _ \<Rightarrow> vl_readers vl \<union> {t})"
-  apply (auto simp add: update_kv_key_reads_defs vl_readers_def in_set_conv_nth split: option.split)
-  subgoal for y ver i by (cases "i = Max (full_view vl)"; simp)
-  apply (rule bexI [where x="update_kv_key_reads t Fk (full_view vl) vl ! Max (full_view vl)"])
-    apply (auto simp add: update_kv_key_reads_defs)
-  subgoal for y ver i apply (cases "i = Max (full_view vl)", simp)
-     apply (metis in_set_update insert_iff max_in_full_view version.select_convs(3)
-        version.surjective version.update_convs(3))
-    by (metis length_list_update nth_list_update_neq nth_mem)
-  done
+*)
 
 
-(************************************)
-(* INTEGRATE STUFF BELOW INTO ABOVE *)
-(************************************)
+subsubsection \<open>Lemmas about readers, writers, and all txids\<close>
 
-
-
-
-
-lemma length_update_kv:
-  "length (update_kv t F u K k) = (if F k W = None then length (K k) else  Suc (length (K k)))"
-  by (auto simp add: update_kv_key_writes_decides_length update_kv_key_writes_def)
-
-
-lemma v_writer_in_kvs_txids:
-  "i < length (K k) \<Longrightarrow> v_writer (K k ! i) \<in> kvs_txids K"
-  by (auto simp add: kvs_txids_def kvs_writers_def vl_writers_def intro: exI[where x=k])
-
-
-(*****)
+text \<open>Writers\<close>
 
 lemma vl_writers_update_kv_key_writes:
-  "vl_writers (update_kv_key_writes t Fk vl) = 
-   (if Fk W = None then vl_writers vl else insert (Tn t) (vl_writers vl))"
-  by (simp add: update_kv_key_writes_def vl_writers_def split: option.split)
+  "vl_writers (update_kv_key_writes t vo vl) = 
+   (if vo = None then vl_writers vl else insert (Tn t) (vl_writers vl))"
+  by (auto simp add: vl_writers_def)
 
-thm update_kv_key_reads_vl_writers_inv
-
-lemma vl_writers_update_kv_key_reads:  (* same as update_kv_key_reads_vl_writers_inv *)
-  "vl_writers (update_kv_key_reads t Fk uk vl) = vl_writers vl"  
-  apply (auto simp add: update_kv_key_reads_def vl_writers_def last_version_def Let_def split: option.split)
-   apply (metis image_eqI list_update_beyond nth_mem the_update verit_comp_simplify1(3) 
-                version.select_convs(2) version.surjective version.update_convs(3))
+lemma vl_writers_update_kv_key_reads:
+  "vl_writers (update_kv_key_reads t vo uk vl) = vl_writers vl"  
+  apply (cases vo)
+  apply (auto simp add: Let_def vl_writers_def)
+   apply (metis (mono_tags, lifting) image_iff list_update_beyond nth_mem the_update 
+                verit_comp_simplify1(3) version.select_convs(2) version.surjective 
+                version.update_convs(3))
   by (metis (mono_tags, lifting) image_iff in_set_after_update list_update_beyond set_update_memI 
-            verit_comp_simplify1(3) version.select_convs(2) version.surjective version.update_convs(3))
-
-lemma vl_readers_update_kv_key_writes:
-  "vl_readers (update_kv_key_writes t Fk vl) = vl_readers vl"
-  by (auto simp add: update_kv_key_writes_def vl_readers_def split: option.split)
-
-lemma vl_readers_update_kv_key_reads:
-  assumes "\<And>v. Fk R = Some v \<Longrightarrow> Max uk < length vl"
-  shows "vl_readers (update_kv_key_reads t Fk uk vl) = 
-         (if Fk R = None then vl_readers vl else insert t (vl_readers vl))"
-  using assms
-  apply (auto simp add: vl_readers_def update_kv_key_reads_simps)
-    apply (metis (no_types, lifting) full_view_def in_set_conv_nth lessThan_iff update_kv_key_reads_length 
-                 update_kv_key_reads_simps(2) v_readerset_update_kv_key_reads_max_u)
-   apply (rule bexI[where x="update_kv_key_reads t Fk uk vl ! Max uk"], 
-          simp add: update_kv_key_reads_simps, simp add: update_kv_key_reads_length)
-  by (smt (verit, best) in_set_after_update insert_iff last_version_def option.case(2) 
-          set_update_memI update_kv_key_reads_defs(1) version.select_convs(3) version.surjective 
-          version.update_convs(3))
-
-
-(***)
-
+      verit_comp_simplify1(3) version.select_convs(2) version.surjective version.update_convs(3))
 
 lemma kvs_writers_update_kv:
-  "kvs_writers (update_kv t fp u K) = 
-   (if \<forall>k. fp k W = None then kvs_writers K else insert (Tn t) (kvs_writers K))"
+  "kvs_writers (update_kv t F u K) = 
+   (if \<forall>k. F k W = None then kvs_writers K else insert (Tn t) (kvs_writers K))"
   by (auto 4 3 simp add: update_kv_def update_kv_key_def kvs_writers_def 
-                         vl_writers_update_kv_key_writes)
+                         vl_writers_update_kv_key_reads vl_writers_update_kv_key_writes)
+
+text \<open>Readers\<close>
+
+lemma vl_readers_update_kv_key_writes:
+  "vl_readers (update_kv_key_writes t vo vl) = vl_readers vl"
+  by (cases vo) (simp_all add: vl_readers_def)
+
+lemma vl_readers_update_kv_key_reads:
+  assumes "\<And>v. vo = Some v \<Longrightarrow> Max uk < length vl"        (* FIX: MODIFY PREMISE *)
+  shows "vl_readers (update_kv_key_reads t vo uk vl) = 
+         (if vo = None then vl_readers vl else insert t (vl_readers vl))"
+  using assms
+  apply (auto simp add: vl_readers_def Let_def)
+  subgoal by (metis insert_iff nth_mem the_update version.select_convs(3) version.surjective 
+                    version.update_convs(3))
+  subgoal by (metis insertCI set_update_memI version.select_convs(3) version.surjective 
+                    version.update_convs(3)) 
+  subgoal by (metis in_set_after_update insert_iff set_update_memI version.select_convs(3) 
+                    version.surjective version.update_convs(3))
+  done
 
 lemma kvs_readers_update_kv:
-  assumes "\<And>k v. fp k R = Some v \<Longrightarrow> Max (u k) < length (K k)"
+  assumes "\<And>k v. fp k R = Some v \<Longrightarrow> Max (u k) < length (K k)"   (* FIX: MODIFY PREMISE *)
   shows "kvs_readers (update_kv t fp u K) = 
          (if \<forall>k. fp k R = None then kvs_readers K else insert t (kvs_readers K))"
   using assms
@@ -1087,7 +1333,30 @@ lemma kvs_readers_update_kv_write_only:
   by (fact kvs_readers_update_kv[where fp="write_only_fp kv_map" for kv_map, simplified])
 
 
+(*******************************)
+(* TODO: integrate stuff below *)
+(*******************************)
 
+lemma update_kv_key_reads_vl_readers_inv:
+  "vl \<noteq> [] \<Longrightarrow> 
+   vl_readers (update_kv_key_reads t vo (full_view vl) vl) =
+   (if vo = None then vl_readers vl else insert t (vl_readers vl))"
+  by (simp add: full_view_elemD vl_readers_update_kv_key_reads)
+
+(*
+  apply (auto simp add: update_kv_key_reads_defs vl_readers_def in_set_conv_nth split: option.split)
+  subgoal for y ver i by (cases "i = Max (full_view vl)"; simp)
+  apply (rule bexI [where x="update_kv_key_reads t Fk (full_view vl) vl ! Max (full_view vl)"])
+    apply (auto simp add: update_kv_key_reads_defs)
+  subgoal for y ver i apply (cases "i = Max (full_view vl)", simp)
+     apply (metis in_set_update insert_iff max_in_full_view version.select_convs(3)
+        version.surjective version.update_convs(3))
+    by (metis length_list_update nth_list_update_neq nth_mem)
+  done
+*)
+
+
+text \<open>All txids in KVS\<close>
 
 lemma kvs_txids_update_kv: 
   assumes "\<And>k v. fp k R = Some v \<Longrightarrow> Max (u k) < length (K k)" 
@@ -1105,10 +1374,11 @@ lemma kvs_txids_update_kv_write_only:
   by (fact kvs_txids_update_kv[where fp="write_only_fp kv_map" for kv_map, simplified])
 
 
-(************************************)
-(************************************)
-(************************************)
+text \<open>Other lemmas\<close>
 
+lemma v_writer_in_kvs_txids:
+  "i < length (K k) \<Longrightarrow> v_writer (K k ! i) \<in> kvs_txids K"
+  by (auto simp add: kvs_txids_def kvs_writers_def vl_writers_def intro: exI[where x=k])
 
 
 end
